\section{Fourier transform of a sum function}

Define a function with summation:

\begin{equation}\label{sum-function-definition}
    F(\mathbf{r}) = \sum_{\mathbf{R}} f(\mathbf{r}+\mathbf{R}) \\
\end{equation}

\noindent
3D case:

\begin{equation}\label{sum-function-fourier-3D}
    \begin{gathered}
        F(\mathbf{r}) = F(\mathbf{r}+\mathbf{R}) 
            = \sum_{\mathbf{k}} F(\mathbf{k}) e^{i\mathbf{k}\cdot\mathbf{r}} , \, 
            e^{i\mathbf{k}\cdot\mathbf{R}} = 1 \\
        \begin{aligned}
            F(\mathbf{k}) 
            &= \frac{1}{\Omega} \int_{\Omega} \mathrm{d}\mathbf{r} \, F(\mathbf{r}) e^{-i\mathbf{k}\cdot\mathbf{r}} \\
            &= \frac{1}{\Omega} \int_{\Omega} \mathrm{d}\mathbf{r} \sum_{\mathbf{R}} f(\mathbf{r}+\mathbf{R}) e^{-i\mathbf{k}\cdot(\mathbf{r}+\mathbf{R})} \\
            &= \frac{1}{\Omega} \int \mathrm{d}\mathbf{r} \, f(\mathbf{r}) e^{-i\mathbf{k}\cdot\mathbf{r}} \\
            &= \frac{1}{\Omega} f(\mathbf{k})
        \end{aligned}
    \end{gathered}
\end{equation}

\noindent
2D case:

\begin{equation}\label{sum-function-fourier-2D}
    \begin{gathered}
        F(\mathbf{r}) = F(x+R_x,y+R_y,z) 
        = \sum_{\mathbf{k}} F(k_x, k_y, z) e^{i(k_x x + k_y y)} , \, 
            e^{i(k_xR_x + k_yR_y)} = 1 \\
        \begin{aligned}
            F(k_x, k_y, z) 
            &= \frac{1}{S} \int_{S} \mathrm{d}x \mathrm{d}y F(\mathbf{r}) e^{-i(k_x x + k_y y)} \\
            &= \frac{1}{S} \int_{S} \mathrm{d}x \mathrm{d}y \sum_{R_xR_y} f(\mathbf{r}+\mathbf{R}) e^{-i\mathbf{k}\cdot(\mathbf{r}+\mathbf{R})} \\
            &= \frac{1}{S} \int \mathrm{d}x \mathrm{d}y f(\mathbf{r}) e^{-i\mathbf{k}\cdot\mathbf{r}} \\
            &= \frac{1}{S} f(\mathbf{k}, z) 
        \end{aligned}
    \end{gathered}
\end{equation}


\noindent
1D case:

\begin{equation}\label{sum-function-fourier-1D}
    \begin{gathered}
        F(\mathbf{r}) = F(x+R_x,y,z) 
        = \sum_{\mathbf{k}} F(k_x, y, z) e^{ik_x x} , \, 
            e^{ik_xR_x} = 1 \\
        \begin{aligned}
            F(k_x, y, z) 
            &= \frac{1}{L} \int_{L} \mathrm{d}x F(\mathbf{r}) e^{-ik_xx} \\
            &= \frac{1}{L} \int_{L} \mathrm{d}x \sum_{R_x} f(\mathbf{r}+\mathbf{R}) e^{-i\mathbf{k}\cdot(\mathbf{r}+\mathbf{R})} \\
            &= \frac{1}{L} \int \mathrm{d}x f(\mathbf{r}) e^{-ik_xx} \\
            &= \frac{1}{L} f(k_x, y, z)
        \end{aligned}
    \end{gathered}
\end{equation}
